examples/boardroomVoting/BoardroomVotingExtractionLiquidity.v
@@ -8,7 +8,7 @@ From ConCert.Extraction Require Import LiquidityExtract.
 From ConCert.Extraction Require Import Common.
 From ConCert.Execution Require Import Blockchain.
 From ConCert.Execution Require Import ContractCommon.
-From ConCert.Execution Require Import LocalBlockchain.
+From ConCert.Execution.Test Require Import LocalBlockchain.
 From ConCert.Examples.BoardroomVoting Require Import BoardroomVotingZ.
 From Coq Require Import ZArith.
 From Coq Require Import List.
@@ -42,7 +42,7 @@ Instance Base : ChainBase := LocalBlockchain.LocalChainBase AddrSize.
 
 Module Params <: BoardroomParams.
   Definition H : list positive -> positive := hash_func.
-  Definition Base := Base .
+  Definition Base := Base.
   Definition prime := modulus.
   Definition generator := generator.
 End Params.  
@@ -89,7 +89,7 @@ Definition receive_wrapper (msg : msg)
   | None => None
   end.
 
-Definition dummy_init : init_ctx -> BV.Setup -> option BV.State := fun _ _ => None .
+Definition dummy_init : init_ctx -> BV.Setup -> option BV.State := fun _ _ => None.
 
 Definition dummy_receive : msg -> BV.State -> option (list ActionBody × BV.State) := 
   fun m s  => 
