examples/congress/tests/CongressPrinters.v
@@ -1,11 +1,8 @@
 From ConCert.Execution Require Import Blockchain.
 From ConCert.Execution Require Import Serializable.
-From ConCert.Execution.QCTest Require Import TestUtils.
-From ConCert.Execution.QCTest Require Import SerializablePrinters.
+From ConCert.Execution.Test Require Import QCTest.
 From ConCert.Examples.Congress Require Import Congress.
-
-From QuickChick Require Import QuickChick. Import QcNotation.
-From Coq Require Import List. Import ListNotations.
+From Coq Require Import List.
 Open Scope string_scope.
 
 Arguments SerializedValue : clear implicits.
@@ -34,7 +31,7 @@ Definition string_of_ca (str_of_msg : Msg -> string) ca :=
 
 Instance showSetup : Show Setup :=
 {|
-  show := show o setup_rules
+  show v := show (setup_rules v)
 |}.
 
 (* Ugly fuel hack :/ *)
