examples/congress/tests/Congress_BuggyGens.v
@@ -2,14 +2,11 @@ From ConCert.Execution Require Import Blockchain.
 From ConCert.Execution Require Import BoundedN.
 From ConCert.Execution Require Import Containers.
 From ConCert.Execution Require Import Serializable.
-From ConCert.Execution.QCTest Require Import TestUtils.
+From ConCert.Execution.Test Require Import QCTest.
 From ConCert.Examples.Congress Require Import Congress_Buggy.
-
-From QuickChick Require Import QuickChick. Import QcNotation.
-Import MonadNotation. Open Scope monad_scope.
-
 From Coq Require Import ZArith.
 From Coq Require Import List. Import ListNotations.
+Import MonadNotation.
 
 Arguments SerializedValue : clear implicits.
 Arguments deserialize : clear implicits.
