examples/dexter/DexterPrinters.v
@@ -1,11 +1,9 @@
 From ConCert.Execution Require Import Blockchain.
 From ConCert.Execution Require Import Serializable.
-From ConCert.Execution.QCTest Require Import TestUtils.
-From ConCert.Execution.QCTest Require Import SerializablePrinters.
+From ConCert.Execution.Test Require Import QCTest.
 From ConCert.Examples.FA2 Require Import FA2Token.
 From ConCert.Examples.FA2 Require Import FA2Printers.
 From ConCert.Examples.Dexter Require Import Dexter.
-From QuickChick Require Import QuickChick.
 
 Local Open Scope string_scope.
 
