examples/eip20/EIP20TokenPrinters.v
@@ -1,9 +1,7 @@
 From ConCert.Execution Require Import Blockchain.
 From ConCert.Execution Require Import Serializable.
+From ConCert.Execution.Test Require Import QCTest.
 From ConCert.Examples Require Import EIP20Token.
-From ConCert.Execution.QCTest Require Import TestUtils.
-From ConCert.Execution.QCTest Require Import SerializablePrinters.
-From QuickChick Require Import QuickChick.
 
 Local Open Scope string_scope.
 
