examples/escrow/Escrow.v
@@ -28,7 +28,7 @@ From ConCert.Utils Require Import Extras.
 From ConCert.Utils Require Import RecordUpdate.
 
 Import ListNotations.
-Import RecordSetNotations.
+
 
 Section Escrow.
 Context `{Base : ChainBase}.
