examples/escrow/tests/EscrowPrinters.v
@@ -2,10 +2,8 @@
 
 From ConCert.Execution Require Import Blockchain.
 From ConCert.Execution Require Import Serializable.
-From ConCert.Execution.QCTest Require Import TestUtils.
-From ConCert.Execution.QCTest Require Import SerializablePrinters.
+From ConCert.Execution.Test Require Import QCTest.
 From ConCert.Examples.Escrow Require Import Escrow.
-From QuickChick Require Import QuickChick.
 
 Local Open Scope string_scope.
 
