examples/fa2/FA2TokenTests.v
@@ -1,29 +1,15 @@
 From ConCert.Execution Require Import Blockchain.
-From ConCert.Execution Require Import BoundedN.
 From ConCert.Execution Require Import Containers.
-From ConCert.Execution Require Import LocalBlockchain.
 From ConCert.Execution Require Import Serializable.
 From ConCert.Execution Require Import ResultMonad.
-From ConCert.Execution.QCTest Require Import TestUtils.
-From ConCert.Execution.QCTest Require Import ChainPrinters.
-From ConCert.Execution.QCTest Require Import TraceGens.
+From ConCert.Execution.Test Require Import QCTest.
 From ConCert.Examples.FA2 Require Import FA2Token.
 From ConCert.Examples.FA2 Require Import FA2Interface.
 From ConCert.Examples.FA2 Require Import TestContracts.
 From ConCert.Utils Require Import Extras.
-From ConCert.Utils Require Import RecordUpdate.
-Global Set Warnings "-extraction-logical-axiom".
-
-From QuickChick Require Import QuickChick. Import QcNotation.
-From ExtLib.Structures Require Import Functor.
-From ExtLib.Structures Require Import Applicative.
-From ExtLib.Structures Require Monads.
-From Coq Require Import Strings.String.
 From Coq Require Import ZArith.
 From Coq Require Import List.
 Import ListNotations.
-Import RecordSetNotations.
-Close Scope address_scope.
 
 (** example policies *)
 
@@ -78,26 +64,26 @@ Definition token_setup (hook_addr : option Address): FA2Token.Setup := {|
 
 |}.
 
-Definition token_contract_base_addr : Address := BoundedN.of_Z_const AddrSize 128%Z.
+Definition token_contract_base_addr : Address := addr_of_Z 128%Z.
 Definition fa2hook_setup : HookSetup := {|
   hook_fa2_caddr_ := token_contract_base_addr;
   hook_policy_ := policy_self_only;
 |}.
 Definition deploy_fa2hook := create_deployment 0 hook_contract fa2hook_setup.
-Definition fa2hook_contract_addr : Address := BoundedN.of_Z_const AddrSize 130%Z.
+Definition fa2hook_contract_addr : Address := addr_of_Z 130%Z.
 
 Definition deploy_fa2token_with_transfer_hook : @ActionBody LocalChainBase :=
-  create_deployment 0 FA2Token.contract (token_setup (Some fa2hook_contract_addr)) .
+  create_deployment 0 FA2Token.contract (token_setup (Some fa2hook_contract_addr)).
 Definition deploy_fa2token_without_transfer_hook : @ActionBody LocalChainBase :=
   create_deployment 0 FA2Token.contract (token_setup None).
 
 Definition token_client_setup := build_clientsetup token_contract_base_addr.
 Definition deploy_fa2token_client : @ActionBody LocalChainBase := create_deployment 0 client_contract token_client_setup.
-Definition client_contract_addr : Address := BoundedN.of_Z_const AddrSize 129%Z.
+Definition client_contract_addr : Address := addr_of_Z 129%Z.
 
 
 Definition chain_with_token_deployed_with_hook : ChainBuilder :=
-  unpack_result (TraceGens.add_block (lcb_initial AddrSize)
+  unpack_result (TraceGens.add_block empty_chain
   [
     build_act creator creator (act_transfer person_1 10);
     build_act creator creator (act_transfer person_2 10);
@@ -108,7 +94,7 @@ Definition chain_with_token_deployed_with_hook : ChainBuilder :=
   ]).
 
 Definition chain_with_token_deployed_without_hook : ChainBuilder :=
-  unpack_result (TraceGens.add_block (lcb_initial AddrSize)
+  unpack_result (TraceGens.add_block empty_chain
   [
     build_act creator creator (act_transfer person_1 10);
     build_act creator creator (act_transfer person_2 10);
@@ -156,34 +142,17 @@ Module TestInfo <: FA2TestsInfo.
   Definition fa2_contract_addr := token_contract_base_addr.
   Definition fa2_client_addr := client_contract_addr.
   Definition fa2_hook_addr := fa2hook_contract_addr.
-  Definition gAddrWithout (ws : list Address) :=
-    let addrs := filter (fun a => negb (existsb (address_eqb a) ws)) test_chain_addrs in   
-    elems_ zero_address addrs.
-  Definition gUniqueAddrPair : GOpt (Address * Address) :=
-    addr1 <- elems_opt test_chain_addrs ;;
-    let addrs := filter (fun a => negb (address_eqb addr1 a)) test_chain_addrs in   
-    addr2 <- elems_opt addrs ;;
-    returnGenSome (addr1, addr2).
-  
-  (* A quick little sanity check that gUniqueAddrPair generator indeed always generates unique pairs *)
-  (* QuickChick (forAll gUniqueAddrPair (fun p => isSomeCheck p (fun '(addr1, addr2) => negb (address_eqb addr1 addr2)))). *)
-  (* +++ Passed 10000 tests (0 discards) *)
+  Definition accounts := test_chain_addrs_5.
 End TestInfo.
 Module MG := FA2Gens.FA2Gens TestInfo. Import MG.
 
-Definition gFA2TokenChain max_acts_per_block cb length := 
-  gChain cb (fun cb _ => gFA2TokenAction cb) length 1 max_acts_per_block.
-
-Definition gFA2ClientChain max_acts_per_block cb length := 
-  gChain cb (fun cb _ => gClientAction cb) length 1 max_acts_per_block.
-
-
-(* Sample (gFA2TokenAction chain_with_transfer_hook). *)
-(* Sample (gFA2TokenChain 1 chain_with_transfer_hook 10). *)
-
-Definition forAllFA2Traces chain n := forAllBlocks n chain (gFA2TokenChain 1).
-Definition forAllFA2TracesStatePairs chain n := forAllChainStatePairs n chain (gFA2TokenChain 1).
-Notation "{{ P }} c {{ Q }} chain" := (pre_post_assertion 7 chain (gFA2TokenChain 1) FA2Token.contract c P Q)( at level 50).
+Module NotationInfo <: TestNotationParameters.
+  Definition gAction := gFA2TokenAction.
+  Definition init_cb := chain_with_transfer_hook.
+End NotationInfo.
+Module TN := TestNotations NotationInfo. Import TN.
+Extract Constant max_acts_per_block => "1".
+(* Sample gChain. *)
 
 Local Open Scope Z_scope.
 Definition transfer_state_update_correct prev_state next_state transfers :=
@@ -239,11 +208,11 @@ Definition post_transfer_correct (chain : Chain) (cctx : ContractCallContext) ol
   | None => checker false
   end.
 
-(* QuickChick ( *)
-(*   {{ msg_is_transfer }} *)
-(*     token_contract_base_addr *)
-(*   {{ post_transfer_correct }} *)
-(*   chain_without_transfer_hook). *)
+(* QuickChick (
+  {{ msg_is_transfer }}
+    token_contract_base_addr
+  {{ post_transfer_correct }}
+  chain_without_transfer_hook). *)
 (* 14 seconds, max size 7, 1 act per block *)
 (* +++ Passed 10000 tests (0 discards) *)
 
@@ -283,7 +252,7 @@ Definition transfer_balances_correct (old_cs new_cs : ChainState) :=
   | None => checker true
   end.
 
-(* QuickChick (forAllFA2TracesStatePairs chain_with_transfer_hook 1 transfer_balances_correct). *)
+(* QuickChick (forAllChainStatePairs transfer_balances_correct). *)
 (* +++ Passed 10000 tests (0 discards) *)
 
 
@@ -350,7 +319,7 @@ Definition transfer_satisfies_policy_P (old_cs new_cs : ChainState) : Checker :=
   | None => checker false
   end.
 
-(* QuickChick (forAllFA2TracesStatePairs chain_with_transfer_hook 10 transfer_satisfies_policy_P). *)
+(* QuickChick (forAllChainStatePairs transfer_satisfies_policy_P). *)
 (* coqtop-stdout:+++ Passed 10000 tests (0 discards) *)
 
 Definition single_update_op_correct (new_state : FA2Token.State) (op : update_operator) :=
@@ -404,11 +373,11 @@ Definition post_last_update_operator_occurrence_takes_effect (chain : Chain) (cc
   | None => checker false
   end.
 
-(* QuickChick ( *)
-(*   {{msg_is_update_operator}} *)
-(*   token_contract_base_addr *)
-(*   {{post_last_update_operator_occurrence_takes_effect}} *)
-(*   chain_without_transfer_hook *)
-(* ). *)
+(* QuickChick (
+  {{msg_is_update_operator}}
+  token_contract_base_addr
+  {{post_last_update_operator_occurrence_takes_effect}}
+  chain_without_transfer_hook
+). *)
 (* 40 secs, max length 7: *)
 (* coqtop-stdout:+++ Passed 10000 tests (0 discards) *)
